proof/Simple_Data/EvJudge.v
@@ -4,6 +4,7 @@ Require Import Preservation.
 Require Import TyJudge.
 Require Export EsJudge.
 Require Export Exp.
+Require Import BaseList.
 
 
 (* Big Step Evaluation **********************************************
@@ -25,11 +26,11 @@ Inductive EVAL : exp -> exp -> Prop :=
    -> EVAL (XApp x1 x2)      v3
 
  | EvCon
-   :  forall dc xs vs v3
-   ,  Forall2 EVAL xs vs
-   -> Forall whnfX vs
-   -> EVAL (XCon dc vs) v3
-   -> EVAL (XCon dc xs) v3
+   :  forall x v v3 dc Cs
+   ,  EVAL x v -> whnfX v
+   -> exps_ctx Cs
+   -> EVAL (XCon dc (Cs v)) v3
+   -> EVAL (XCon dc (Cs x)) v3
 
  | EvCase 
    :  forall x1 x2 v3 dc vs alts tsArgs
@@ -60,163 +61,89 @@ Hint Resolve eval_produces_whnfX.
    machine steps.
  *)
 
-Lemma steps_of_evals
- :  forall ds xs ts vs 
- ,  Forall2 (TYPE ds Empty) xs ts
- -> Forall2 EVAL  xs vs
- -> Forall2 STEPS xs vs.
-Proof.
- admit.
-Qed.
 
-Lemma steps_con
+(* Reduce one of the arguments to a data constructor. 
+   The definition of evaluation contexts enforces a left-to-right 
+   order of evaluation, so all the arguments to the left of the one
+   to be reduced already need to be values. *)
+Lemma steps_context_XCon
  :  forall ix x v vs xs xs' dc
- ,  Forall value vs
- -> STEPS x v
- -> splitAt ix xs = (vs, x :: xs')
+ ,  splitAt ix xs = (vs, x :: xs')
+ -> Forall value vs
+ -> STEPS  x v
  -> STEPS (XCon dc xs) (XCon dc (vs ++ (v :: xs'))).
 Proof.
  intros.
  lets D: steps_context XcCon. eapply (XscIx ix). eauto. auto.
- lets D1: D H0. clear D.
-  assert (xs = app vs (x :: xs')). skip.
+ lets D1: D H1. clear D.
+  assert (xs = app vs (x :: xs')). eapply splitAt_app. eauto.
    rewrite H2.
  apply D1.
 Qed.
 
 
-Lemma steps_con3
- :  forall ix vs xs xs' vs' dc x v acc
- ,  Forall  value vs 
- -> STEPS   x v             -> value v
- -> Forall2 STEPS xs' vs'   -> Forall  value vs'
- -> splitAt ix acc xs = Some (app acc vs, x :: xs')
- -> STEPS (XCon dc xs) (XCon dc (vs ++ (v :: vs'))).
-Proof.
- intros. gen x v xs xs' vs vs' acc.
- induction ix; intros.
-
- Case "ix = 0".
-  admit.
-
- Case "ix = S ix'".
-  assert (xs = app vs (x :: xs')). admit. (* prop splitAt *)
-  rewrite H5.
-
-  (* do the first eval *)
-  eapply EsAppend.
-   lets D: steps_context XcCon. 
-    eapply XscIx with (ix := List.length vs)
-                      (vs := vs).
-    skip. 
-    auto.
-   lets D1: D H0. eapply D1.
-
-  (* do the rest, need to reassociate ++ *)
-  destruct vs' as [vs2 | v2].
-   SCase "vs' = nil".
-    inverts H2. auto.
-
-   SCase "vs' = vs2 :: v2".
-    assert (app vs (v :: v2 :: vs') = app (app vs (v :: nil)) (v2::vs')).
-     admit.
-    rewrite H6.
-
-   inverts H2.
-   eapply IHix.
-    eauto.
-    inverts H3. eauto.
-    admit. (* ok *)
-    eauto.
-    inverts H3. eauto. clear IHix.
-    rewrite H5 in H4.
-
-    assert ( splitAt ix nil (app vs (v :: x0 :: l0))
-           = Some (app nil (app vs (v :: nil)), x0 :: l0)).
-     simpl.
-
-    (* we've gone the wrong way wirh the rewrite *)
-    (* almosted worked though.
-        splitAt ix acc (acc ++ xx, yy) => ix == length ix
-       this is all the info we should need from the hyp 
-      
-       do more lemmas involving splitAt
-       maybe better to use:
-       splitAt ix xx = (take ix xx, drop ix xx)
-
-       .. or not, because we don't want ix in the right
-       of the definition. Just do this as a lemma.
-     *)
-
-    admit.
-    eapply H2.
-
- 
- (********* junk *)
-  admit.
-
-  assert (xs = app vs xs'). admit. rewrite H3. clear H3.
- 
-  destruct xs'.
-   admit.
-   eapply EsAppend.
-    lets D: steps_context XcCon. eapply XscIx. eauto. eauto.
-    destruct vs'.
-     inverts H0.
-     inverts H0.
-      eapply D. eauto.
-
-
-   assert (xs = app vs (e :: xs')). admit. (* ok, prop of splitAt *)
-   eapply EsAppend.
-   inverts H0.
-    eapply steps_con4 
-      with (xs' := xs') (ix  := S ix) (x := e). eauto. eauto.
-    
-     rewrite <- H3. 
-      assert (app nil vs = vs). simpl. auto.
-      rewrite <- H0 in H2. eauto.
-      simpl. 
-      rewrite <- H3. clear H3.
-
-      destruct xs'.
-       admit.
-       assert (splitAt ix nil xs = Some (app vs (e :: nil), e0:: xs')).
-        admit. clear H2.
-
-      destruct vs'  as [vs2 | v0]. inverts H0.
-      destruct vs'  as [vs3 | v1]. inverts H0. inverts H8.
-     
-      assert (xs = app vs (e :: e0 :: xs')).
-       admit. rewrite H2.
-
-     eapply EsAppend.
-     eapply IHix.
-      eauto. rewrite <- H2. eauto.
-
-      
-
-Lemma steps_con
- : forall xs vs dc 
- ,  Forall2 STEPS xs vs 
- -> Forall  value vs
- -> STEPS (XCon dc xs) (XCon dc vs).
+Lemma steps_context_XCon_2 
+ :   forall v x dc Cs
+ ,   STEPS x v
+ ->  exps_ctx Cs
+ ->  STEPS (XCon dc (Cs x)) (XCon dc (Cs v)).
 Proof.
  intros.
- induction vs.
-  inverts H. auto.
-
-  destruct xs. 
-   inverts H.
-
-   assert (a :: vs = app nil (a :: vs)). 
-    simpl. auto. rewrite H1. clear H1.
-   eapply (steps_con3 0 e a) with (xs' := xs). simpl. auto.
-   auto.
-   inverts H. auto.
-   inverts H. auto.
+ lets D: steps_context XcCon. eauto.
+ eauto.
 Qed.
- 
+
+
+Lemma Forall2_exists_left_In
+ : forall (A B: Type) (R: A -> B -> Prop) x xs ys
+ ,             In x xs  -> Forall2 R xs ys 
+ -> (exists y, In y ys  /\         R x  y).
+Proof.
+ intros.
+ induction H0.
+  false.
+  simpl in H. destruct H.
+   subst.
+   exists y. split. simpl. auto. auto.
+   lets D: IHForall2 H.
+   destruct D.
+   exists x1.
+    inverts H2.
+    split. simpl. auto. auto.
+Qed.
+
+
+Lemma exps_ctx_Forall2 
+ :   forall {B: Type} (R: exp -> B -> Prop) 
+            (x: exp)  Cs
+            (y: B)    (ys: list B)
+ ,   exps_ctx Cs
+ ->  Forall2 R (Cs x) ys
+ ->  (exists y, In y ys /\ R x y).
+Proof.
+ intros.
+ inverts H.
+ assert (In x (vs ++ x :: xs')).
+  admit.
+ lets D: Forall2_exists_left_In H H0.
+ destruct D. 
+ exists x1. eauto.
+Qed.  
+
+
+Lemma exps_ctx_Forall2_swap
+ :   forall {B: Type} (R: exp -> B -> Prop)
+            (x1 x2 : exp) Cs
+            (y: B)        (ys: list B)
+ ,   exps_ctx Cs
+ ->  R x1 y
+ ->  R x2 y
+ ->  Forall2 R (Cs x1) ys
+ ->  Forall2 R (Cs x2) ys.
+Proof.
+ admit.
+Qed.
+
 
 Lemma steps_of_eval
  :  forall ds x1 t1 x2
@@ -253,15 +180,22 @@ Proof.
 
  Case "EvCon".
   intros. inverts keep HT.
-  lets D: steps_of_evals H. eauto.
-   eapply steps_con. eauto.
-    admit. (* ok, vs values *)
-    eapply IHHE. eauto.
-    eapply TYCon. eauto.
-    admit. (* ok, vs well typed *)
 
+  lets HTx: (@exps_ctx_Forall2 ty) H0 H7. auto.
+  destruct HTx as [t]. inverts H1.
+
+  lets HSx: IHHE1 H3. clear IHHE1.
+  lets HTv: preservation_steps H3 HSx.
+
+  eapply EsAppend.
+   lets D: steps_context XcCon. eauto.
+    eapply D. eapply HSx.
+
+   eapply IHHE2.
+   eapply TYCon. eauto.
+   eapply exps_ctx_Forall2_swap.
+    eauto. eapply H3. eauto. eauto.
   
-
  Case "EvCase".
   intros. inverts keep HT.
 
@@ -332,7 +266,7 @@ Proof.
     inverts HT. inverts H0. inverts H1. eauto.
 
    SCase "XcCon".
-    inverts HT. inverts H0. inverts H1.
+    inverts HT. 
     admit. (********* TODO: need big step rule *)
 
    SCase "XcCase".
